Split the LLBC+ and LLBC# semantics into two files.

src/LLBC_sharp.v
@@ -1,9 +1,8 @@
-(** * Mechanized_LLBC.LLBC_sharp : Semantics of LLBC+ and LLBC#. *)
-From stdpp Require Import pmap gmap.
-Require Import base OptionMonad PathToSubtree SimulationUtils lang.
+(** * Mechanized_LLBC.LLBC_sharp : Semantics of LLBC#. *)
+From stdpp Require Import fin_maps.
+Require Import base PathToSubtree SimulationUtils lang.
 Require Import Symbolic_states Symbolic_relations.
 
-(** * Semantics of LLBC## *)
 Inductive eval_proj (S : state) perm : proj -> spath -> spath -> Prop :=
 (* Coresponds to R-Deref-MutBorrow and W-Deref-MutBorrow in the article. *)
 | E_Deref_MutBorrow q l
@@ -27,27 +26,6 @@ Definition eval_place S perm (p : place) pi :=
 Global Notation "S  |-{p}  p =>^{ perm } pi" := (eval_place S perm p pi)
   (at level 50) : llbc_sharp_scope.
 
-Lemma eval_proj_valid S perm proj q r (H : eval_proj S perm proj q r) : valid_spath S r.
-Proof.
-  induction H.
-  - apply valid_spath_app. split.
-    + apply get_not_bot_valid_spath. destruct (S.[q]); discriminate.
-    + destruct (S.[q]); inversion get_q. econstructor; reflexivity || constructor.
-Qed.
-
-Lemma eval_path_valid (s : state) P perm q r
-  (valid_q : valid_spath s q) (eval_q_r : eval_path s perm P q r) :
-  valid_spath s r.
-Proof.
-  induction eval_q_r.
-  - assumption.
-  - apply IHeval_q_r. eapply eval_proj_valid. eassumption.
-Qed.
-
-Lemma eval_place_valid s p perm pi (H : eval_place s perm p pi) : valid_spath s pi.
-Proof. destruct H as (? & ?). eapply eval_path_valid; eassumption. Qed.
-Hint Resolve eval_place_valid : spath.
-
 Definition copiable (ty : LLBC_type) := True.
 
 Inductive copy_val : value -> value -> Prop :=
@@ -61,12 +39,12 @@ Variant eval_operand : operand -> state -> (value * state) -> Prop :=
 | E_IntConst S n : S |-{op} Const (IntConst n) => (VInt n, S)
 | E_BoolConst S b : S |-{op} Const (BoolConst b) => (VBool b, S)
 | E_Copy S (p : place) pi v
-    (Heval_place : eval_place S Imm p pi) (Hcopy_val : copy_val (S.[pi]) v) :
+    (Heval_place : S |-{p} p =>^{Imm} pi) (Hcopy_val : copy_val (S.[pi]) v) :
     S |-{op} Copy p => (v, S)
-| E_Move S (p : place) pi (Heval : eval_place S Mov p pi)
+| E_Move S (p : place) pi (Heval : S |-{p} p =>^{Mov} pi)
     (move_no_loan : not_contains_loan (S.[pi])) (move_no_bot : not_contains_bot (S.[pi])) :
     S |-{op} Move p => (S.[pi], S.[pi <- bot])
-where "S |-{op} op => r" := (eval_operand op S r) : llbc_sharp_scope.
+where "S  |-{op}  op  =>  r" := (eval_operand op S r) : llbc_sharp_scope.
 
 Variant eval_binary_op : BinOp -> value -> value -> value -> Prop :=
   | E_Add_int_int m n :
@@ -103,7 +81,7 @@ Variant eval_rvalue : rvalue -> state -> (value * state) -> Prop :=
       (fresh_l : is_fresh l S)
       (Htype : is_of_type ty (S.[pi])) :
       S |-{rv} (&mut p) => (borrow^m(l, S.[pi]), S.[pi <- loan^m(ty, l)])
-where "S |-{rv} rv => r" := (eval_rvalue rv S r) : llbc_sharp_scope.
+where "S  |-{rv}  rv  =>  r" := (eval_rvalue rv S r) : llbc_sharp_scope.
 
 (* Note: we use the variable names i' and j' instead of i and j that are used for leq_state_base.
  * We are also using the name A' instead of A, B or C for the region abstractions.
@@ -148,99 +126,47 @@ Variant store (p : place) : value * state -> state -> Prop :=
 (** We simply need to rename the tags of each branch. *)
 Definition end_loop (B : branching_state) : branching_state := pkmap end_loop_tag B.
 
-Inductive LLBC_plus_eval_stmt : nat -> statement -> state -> branching_state -> Prop :=
-  | LLBC_plus_E_Step_Zero s S : S |-{stmt} s ~>{0} empty
-  | LLBC_plus_E_Nop n S : S |-{stmt} Nop ~>{1 + n} {[rUnit := S]}
-  | LLBC_plus_E_Panic n S : S |-{stmt} Panic ~>{1 + n} {[rPanic := S]}
-  | LLBC_plus_E_Break n S : S |-{stmt} Break ~>{1 + n} {[rBreak := S]}
-  | LLBC_plus_E_Continue n S : S |-{stmt} Continue ~>{1 + n} {[rContinue := S]}
-  | LLBC_plus_E_Seq_Propagate n S0 B1 stmt_0 stmt_1
-      (eval_stmt_0 : S0 |-{stmt} stmt_0 ~>{1 + n} B1) (Hno_unit : lookup rUnit B1 = None) :
-      S0 |-{stmt} (Seq stmt_0 stmt_1) ~>{1 + n} B1
-  | LLBC_plus_E_Seq_Unit_Propagate n S0 B1 S_unit B_unit B_join stmt_0 stmt_1
-      (eval_stmt_0 : S0 |-{stmt} stmt_0 ~>{1 + n} B1)
-      (H_unit : lookup rUnit B1 = Some S_unit)
-      (eval_stmt_1 : S_unit |-{stmt} stmt_1 ~>{1 + n} B_unit)
-      (His_join : is_join B_unit (delete rUnit B1) B_join) :
-      S0 |-{stmt} (Seq stmt_0 stmt_1) ~>{1 + n} B_join
-  | LLBC_plus_E_Assign n S vS' S'' p rv (eval_rv : S |-{rv} rv => vS') (Hstore : store p vS' S'') :
-      S |-{stmt} ASSIGN p <- rv ~>{1 + n} {[rUnit := S'']}
-  | LLBC_plus_E_IfThenElse_T n S S' B_if cond stmt_if stmt_else
-      (eval_cond : S |-{op} cond => (VBool true, S'))
-      (Heval_if_branch : S' |-{stmt} stmt_if ~>{1 + n} B_if) :
-      S |-{stmt} (IF cond {{ stmt_if }} ELSE {{ stmt_else }}) ~>{1 + n} B_if
-  | LLBC_plus_E_IfThenElse_F n S S' B_else cond stmt_if stmt_else
-      (eval_cond : S |-{op} cond => (VBool false, S'))
-      (Heval_else_branch : S' |-{stmt} stmt_else ~>{1 + n} B_else) :
-      S |-{stmt} (IF cond {{ stmt_if }} ELSE {{ stmt_else }}) ~>{1 + n} B_else
-  (* Note: in the ICFP'24 article, the symbolic value is replaced by a concrete boolean in each
-     branch. We cannot do that as symbolic values are currently not named. *)
-  | LLBC_plus_IfThenElse_Symbolic n S S' B_if B_else B_join cond stmt_if stmt_else
-      (eval_cond : S |-{op} cond => (VSymbolic TBool, S'))
-      (Heval_if_branch : S' |-{stmt} stmt_if ~>{1 + n} B_if)
-      (Heval_else_branch : S' |-{stmt} stmt_else ~>{1 + n} B_else)
-      (His_join : is_join B_if B_else B_join) :
-      S |-{stmt} (IF cond {{ stmt_if }} ELSE {{ stmt_else }}) ~>{1 + n} B_join
-  | LLBC_plus_E_Reorg n S0 S1 B2 stmt (Hreorg : reorg^* S0 S1) (Heval : S1 |-{stmt} stmt ~>{1 + n} B2) :
-      S0 |-{stmt} stmt ~>{1 + n} B2
-  (* We perform a single loop iteration, and stop because it does not continue. *)
-  | LLBC_plus_E_Loop_Stop n S body B1
-      (eval_body : S |-{stmt} body ~>{1 + n} B1)
-      (* An iteration that yields `rUnit` gets stuck. *)
-      (no_unit : lookup rUnit B1 = None)
-      (no_continue : lookup rContinue B1 = None) :
-      S |-{stmt} (LOOP {{ body }}) ~>{1 + n} (end_loop B1)
-  | LLBC_plus_E_Loop_Continue n S body B1 S1 B2 Bend
-      (eval_body : S |-{stmt} body ~>{1 + n} B1)
-      (* An iteration that yields `rUnit` gets stuck. *)
-      (no_unit : lookup rUnit B1 = None)
-      (Hcontinue : lookup rContinue B1 = Some S1)
-      (Heval2 : S1 |-{stmt} (LOOP {{ body }}) ~>{n} B2)
-      (His_join : is_join (end_loop (delete rContinue B1)) B2 Bend) :
-      S |-{stmt} (LOOP {{ body }}) ~>{1 + n} Bend
-where "S |-{stmt} stmt ~>{ n } B" := (LLBC_plus_eval_stmt n stmt S B) : llbc_sharp_scope.
-
-Inductive LLBC_sharp_eval_stmt : statement -> state -> branching_state -> Prop :=
-  | LLBC_sharp_E_Nop S : S |-# Nop ~> {[rUnit := S]}
-  | LLBC_sharp_E_Panic S : S |-# Panic ~> {[rPanic := S]}
-  | LLBC_sharp_E_Break S : S |-# Break ~> {[rBreak := S]}
-  | LLBC_sharp_E_Continue S : S |-# Continue ~> {[rContinue := S]}
-  | LLBC_sharp_E_Seq_Propagate S0 B1 stmt_0 stmt_1
+Inductive eval_stmt : statement -> state -> branching_state -> Prop :=
+  | E_Nop S : S |-# Nop ~> {[rUnit := S]}
+  | E_Panic S : S |-# Panic ~> {[rPanic := S]}
+  | E_Break S : S |-# Break ~> {[rBreak := S]}
+  | E_Continue S : S |-# Continue ~> {[rContinue := S]}
+  | E_Seq_Propagate S0 B1 stmt_0 stmt_1
       (eval_stmt_0 : S0 |-# stmt_0 ~> B1) (Hno_unit : lookup rUnit B1 = None) :
       S0 |-# (Seq stmt_0 stmt_1) ~> B1
-  | LLBC_sharp_E_Seq_Unit_Propagate S0 B1 S1 B2 stmt_0 stmt_1
+  | E_Seq_Unit_Propagate S0 B1 S1 B2 stmt_0 stmt_1
       (eval_stmt_0 : S0 |-# stmt_0 ~> B1)
       (H_unit : lookup rUnit B1 = Some S1)
       (leq_B1_B2 : leq_branching (delete rUnit B1) B2)
       (eval_stmt_1 : S1 |-# stmt_1 ~> B2) :
       S0 |-# (Seq stmt_0 stmt_1) ~> B2
-  | LLBC_sharp_E_Assign S vS' S'' p rv (eval_rv : S |-{rv} rv => vS') (Hstore : store p vS' S'') :
+  | E_Assign S vS' S'' p rv (eval_rv : S |-{rv} rv => vS') (Hstore : store p vS' S'') :
       S |-# ASSIGN p <- rv ~> {[rUnit := S'']}
-  | LLBC_sharp_E_IfThenElse_T S S' B_if cond stmt_if stmt_else
+  | E_IfThenElse_T S S' B_if cond stmt_if stmt_else
       (eval_cond : S |-{op} cond => (VBool true, S'))
       (Heval_if_branch : S' |-# stmt_if ~> B_if) :
       S |-# (IF cond {{ stmt_if }} ELSE {{ stmt_else }}) ~> B_if
-  | LLBC_sharp_E_IfThenElse_F S S' B_else cond stmt_if stmt_else
+  | E_IfThenElse_F S S' B_else cond stmt_if stmt_else
       (eval_cond : S |-{op} cond => (VBool false, S'))
       (Heval_else_branch : S' |-# stmt_else ~> B_else) :
       S |-# (IF cond {{ stmt_if }} ELSE {{ stmt_else }}) ~> B_else
   (* Note: in the ICFP'24 article, the symbolic value is replaced by a concrete boolean in each
      branch. We cannot do that as symbolic values are currently not named. *)
-  | LLBC_sharp_IfThenElse_Symbolic S S' B cond stmt_if stmt_else
+  | E_IfThenElse_Symbolic S S' B cond stmt_if stmt_else
       (eval_cond : S |-{op} cond => (VSymbolic TBool, S'))
       (Heval_if_branch : S' |-# stmt_if ~> B)
       (Heval_else_branch : S' |-# stmt_else ~> B) :
       S |-# (IF cond {{ stmt_if }} ELSE {{ stmt_else }}) ~> B
-  | LLBC_sharp_E_Reorg S0 S1 B2 stmt (Hreorg : reorg^* S0 S1) (Heval : S1 |-# stmt ~> B2) :
+  | E_Reorg S0 S1 B2 stmt (Hreorg : reorg^* S0 S1) (Heval : S1 |-# stmt ~> B2) :
       S0 |-# stmt ~> B2
   (* We perform a single loop iteration, and stop because it does not continue. *)
-  | LLBC_sharp_E_Loop_Stop S body B1
+  | E_Loop_Stop S body B1
       (eval_body : S |-# body ~> B1)
       (* An iteration that yields `rUnit` gets stuck. *)
       (no_unit : lookup rUnit B1 = None)
       (no_continue : lookup rContinue B1 = None) :
       S |-# (LOOP {{ body }}) ~> (end_loop B1)
-  | LLBC_sharp_E_Loop_Continue S0 body B1 S1 Bend
+  | E_Loop_Continue S0 body B1 S1 Bend
       (eval_body : S0 |-# body ~> B1)
       (* An iteration that yields `rUnit` gets stuck. *)
       (no_unit : lookup rUnit B1 = None)
@@ -249,15 +175,15 @@ Inductive LLBC_sharp_eval_stmt : statement -> state -> branching_state -> Prop :
       (Heval2 : S1 |-# (LOOP {{ body }}) ~> Bend) :
        S0 |-# (LOOP {{ body }}) ~> Bend
   (* These are LLBC## only rules. *)
-  | LLBC_sharp_E_Loop_Invariant body Sinv Binv
+  | E_Loop_Invariant body Sinv Binv
       (eval_body : Sinv |-# body ~> Binv)
       (inv_preservation : lookup rContinue Binv = Some Sinv)
       (no_unit : lookup rUnit Binv = None) :
       Sinv |-# (LOOP {{ body }}) ~> (end_loop (delete rContinue Binv))
-  | LLBC_sharp_Weaken_Precondition s Sl Sr B
+  | Consequence_Precondition s Sl Sr B
       (Hweaken : leq_symbolic Sl Sr) (Heval : Sr |-# s ~> B) :
       Sl |-# s ~> B
-  | LLBC_sharp_Weaken_Postcondition s S Bl Br
+  | Consequence_Postcondition s S Bl Br
       (Heval : S |-# s ~> Bl) (Hweaken : leq_branching Bl Br) :
       S |-# s ~> Br
-where "S |-# stmt ~> B" := (LLBC_sharp_eval_stmt stmt S B) : llbc_sharp_scope.
+where "S |-# stmt ~> B" := (eval_stmt stmt S B) : llbc_sharp_scope.
